IykykExamples.lean
@@ -3,3 +3,4 @@ module
 public import Iykyk.Examples.Graph
 public import Iykyk.Examples.Bounded
 public import Iykyk.Examples.Automation
+public import Iykyk.Examples.Certified
